src/Distributions/Uniform/Interface.dfy
@@ -19,18 +19,18 @@ module UniformInterface {
       decreases *
       requires n > 0
       ensures u < n
-      ensures Model.ProbUniform(n)(old(s)) == (u, s)
+      ensures Model.UniformSample(n)(old(s)) == (u, s)
 
     method UniformIntervalSample(a: int, b: int) returns (u: int)
       modifies this
       decreases *
       requires a < b
       ensures a <= u < b
-      ensures Model.ProbUniformInterval(a, b)(old(s)) == (u, s)
+      ensures Model.UniformIntervalSample(a, b)(old(s)) == (u, s)
     {
       var v := UniformSample(b - a);
-      assert Model.ProbUniform(b-a)(old(s)) == (v, s);
-      assert Model.ProbUniformInterval(a, b)(old(s)) == (a + v, s);
+      assert Model.UniformSample(b-a)(old(s)) == (v, s);
+      assert Model.UniformIntervalSample(a, b)(old(s)) == (a + v, s);
       u := a + v;
     }
 
